go back to f268dad72024608dbb3d7c557cb4a94ae5467f08 Dsub.v

stable/Dsub.v
@@ -155,57 +155,47 @@ Inductive okt : env -> Prop :=
 
 (** Subtyping relation *)
 
-Inductive sub_mode : Set :=
-  | notrans : sub_mode
-  | oktrans : sub_mode.
-
-Inductive sub : sub_mode -> env -> typ -> typ -> Prop :=
+Inductive sub : env -> typ -> typ -> Prop :=
   | sub_top : forall E S,
       okt E ->
       wft E S ->
-      sub notrans E S typ_top
+      sub E S typ_top
   | sub_refl_sel : forall E t,
       okt E ->
       wft E (typ_sel t) ->
-      sub notrans E (typ_sel t) (typ_sel t)
-  | sub_sel1 : forall E U t,
-      has E t (typ_mem false U) ->
-      sub notrans E (typ_sel t) U
-  | sub_sel2 : forall E S S1 t,
-      has E t (typ_mem true S1) ->
-      sub oktrans E S S1 ->
-      sub notrans E S (typ_sel t)
-  | sub_mem_false : forall E b1 T1 T2,
-      sub oktrans E T1 T2 ->
-      sub notrans E (typ_mem b1 T1) (typ_mem false T2)
-  | sub_mem_true : forall E T1 T2,
-      sub oktrans E T1 T2 -> sub oktrans E T2 T1 ->
-      sub notrans E (typ_mem true T1) (typ_mem true T2)
-  | sub_all : forall L E S1 S2 T1 T2,
-      sub oktrans E T1 S1 ->
-      (forall x, x \notin L ->
-          sub oktrans (E & x ~ T1) (S2 open_t_var x) (T2 open_t_var x)) ->
-      sub notrans E (typ_all S1 S2) (typ_all T1 T2)
-  | sub_trans_ok : forall E T1 T2,
-      sub notrans E T1 T2 ->
-      sub oktrans E T1 T2
-  | sub_trans_axiom : forall E T1 T2 T3,
-      sub notrans E T1 T2 ->
-      sub oktrans E T2 T3 ->
-      sub oktrans E T1 T3
-
-with has : env -> trm -> typ -> Prop :=
-  | has_var : forall E x T,
-      okt E ->
+      sub E (typ_sel t) (typ_sel t)
+  | sub_sel1 : forall T E U x,
       binds x T E ->
-      has E (trm_fvar x) T
-  | has_mem : forall E T,
-      okt E -> wft E T ->
-      has E (trm_mem T) (typ_mem true T)
-  | has_sub : forall E p T U,
-      has E p T ->
-      sub notrans E T U ->
-      has E p U
+      sub E T (typ_mem false U) ->
+      sub E (typ_sel (trm_fvar x)) U
+  | sub_sel2 : forall T E S S1 x,
+      binds x T E ->
+      sub E T (typ_mem true S1) ->
+      sub E S S1 ->
+      sub E S (typ_sel (trm_fvar x))
+  | sub_selc1 : forall U E T,
+      sub E U T ->
+      sub E (typ_sel (trm_mem U)) T
+  | sub_selc2 : forall S E T,
+      sub E T S ->
+      sub E T (typ_sel (trm_mem S))
+  | sub_mem_false : forall E b1 T1 T2,
+      sub E T1 T2 ->
+      sub E (typ_mem b1 T1) (typ_mem false T2)
+  | sub_mem_true : forall E T1 T2,
+      sub E T1 T2 -> sub E T2 T1 ->
+      sub E (typ_mem true T1) (typ_mem true T2)
+  | sub_all : forall L E S1 S2 T1 T2,
+      sub E T1 S1 ->
+      (forall x, x \notin L ->
+          sub (E & x ~ T1) (S2 open_t_var x) (T2 open_t_var x)) ->
+      sub E (typ_all S1 S2) (typ_all T1 T2)
+(*
+  | sub_trans : forall E T1 T2 T3,
+      sub E T1 T2 ->
+      sub E T2 T3 ->
+      sub E T1 T3
+*)
 .
 
 (** Typing relation *)
@@ -231,7 +221,7 @@ Inductive typing : env -> trm -> typ -> Prop :=
       typing E (trm_app e1 e2) T2'
   | typing_sub : forall S E e T,
       typing E e S ->
-      sub oktrans E S T ->
+      sub E S T ->
       typing E e T.
 
 (** One-step reduction *)
@@ -353,8 +343,7 @@ Ltac get_env :=
   match goal with
   | |- wft ?E _ => E
   | |- wfe ?E _ => E
-  | |- sub _ ?E _ _  => E
-  | |- has ?E _ _ => E
+  | |- sub ?E _ _  => E
   | |- typing ?E _ _ => E
   end.
 
@@ -379,10 +368,6 @@ Combined Scheme lc_mutind from type_mut, term_mut.
 Scheme wft_mut := Induction for wft Sort Prop
 with wfe_mut := Induction for wfe Sort Prop.
 Combined Scheme wf_mutind from wft_mut, wfe_mut.
-
-Scheme sub_mut := Induction for sub Sort Prop
-with has_mut := Induction for has Sort Prop.
-Combined Scheme sub_has_mutind from sub_mut, has_mut.
 
 (* ********************************************************************** *)
 (** * Properties of Substitutions *)
@@ -844,41 +829,29 @@ Qed.
 
 (** The subtyping relation is restricted to well-formed objects. *)
 
-Lemma sub_has_regular : (forall m E S T,
-  sub m E S T -> okt E /\ wft E S /\ wft E T) /\ (forall E p T,
-  has E p T -> okt E /\ wft E (typ_sel p) /\ wft E T).
+Lemma sub_regular : forall E S T,
+  sub E S T -> okt E /\ wft E S /\ wft E T.
 Proof.
-  apply sub_has_mutind; intros; try auto*.
-  splits*. destruct H as [? [? A]]. inversion A; subst. assumption.
+  induction 1; try auto*.
+  splits*. destruct IHsub as [? [? Hmem]]. inversion Hmem; subst. assumption.
+  splits*. apply* wft_sel. left. apply value_mem. apply* wfe_term.
+  splits*. apply* wft_sel. left. apply value_mem. apply* wfe_term.
   split. auto*. split;
    apply_fresh* wft_all as Y;
-    forwards~: (H0 Y); apply_empty* (@wft_narrow T1).
-  splits*. apply wft_sel. left. apply value_mem. apply* wfe_term. apply* wfe_mem.
-Qed.
-
-Lemma sub_regular : forall m E S T,
-  sub m E S T -> okt E /\ wft E S /\ wft E T.
-Proof.
-  intros. apply* (proj1 sub_has_regular).
-Qed.
-
-Lemma wft_has_sel : forall E p T, has E p T -> wft E (typ_sel p).
-Proof.
-  intros. apply (proj2 sub_has_regular) in H. destruct H as [? [? ?]].
-  auto.
+    forwards~: (H1 Y); apply_empty* (@wft_narrow T1).
 Qed.
 
 (** The typing relation is restricted to well-formed objects. *)
 
 Lemma typing_regular : forall E e T,
-  typing E e T -> okt E /\ wfe E e /\ wft E T.
+  typing E e T -> okt E /\ term e /\ wft E T.
 Proof.
   induction 1.
   splits*.
   splits.
    pick_fresh y. specializes H0 y. destructs~ H0.
     forwards*: okt_push_inv.
-   apply_fresh* wfe_abs as y.
+   apply_fresh* term_abs as y.
      pick_fresh y. forwards~ K: (H0 y). destructs K.
        forwards*: okt_push_inv.
      forwards~ K: (H0 y). destructs K. auto.
@@ -887,7 +860,7 @@ Proof.
       forwards*: okt_push_inv.
      forwards~ K: (H0 Y). destructs K.
       forwards*: okt_push_inv.
-  splits*.
+  splits*. apply term_mem. apply* wft_type.
   splits*.
   splits*. destructs~ (sub_regular H0).
 Qed.
@@ -913,23 +886,23 @@ Qed.
 
 Hint Extern 1 (okt ?E) =>
   match goal with
-  | H: sub _ _ _ _ |- _ => apply (proj31 (sub_regular H))
+  | H: sub _ _ _ |- _ => apply (proj31 (sub_regular H))
   | H: typing _ _ _ |- _ => apply (proj31 (typing_regular H))
   end.
 
 Hint Extern 1 (wft ?E ?T) =>
   match goal with
   | H: typing E _ T |- _ => apply (proj33 (typing_regular H))
-  | H: sub _ E T _ |- _ => apply (proj32 (sub_regular H))
-  | H: sub _ E _ T |- _ => apply (proj33 (sub_regular H))
+  | H: sub E T _ |- _ => apply (proj32 (sub_regular H))
+  | H: sub E _ T |- _ => apply (proj33 (sub_regular H))
   end.
 
 Hint Extern 1 (type ?T) =>
   let go E := apply (@wft_type E); auto in
   match goal with
   | H: typing ?E _ T |- _ => go E
-  | H: sub _ ?E T _ |- _ => go E
-  | H: sub _ ?E _ T |- _ => go E
+  | H: sub ?E T _ |- _ => go E
+  | H: sub ?E _ T |- _ => go E
   end.
 
 Hint Extern 1 (term ?e) =>
@@ -956,9 +929,8 @@ Hint Extern 1 (term ?e) =>
 Lemma sub_reflexivity : forall E T,
   okt E ->
   wft E T ->
-  sub notrans E T T .
+  sub E T T .
 Proof.
-  Hint Resolve sub_trans_ok.
   introv Ok WI. lets W: (wft_type WI). gen E.
   induction W; intros; inversions WI; eauto.
   destruct b. apply* sub_mem_true. apply* sub_mem_false.
@@ -968,38 +940,26 @@ Qed.
 (* ********************************************************************** *)
 (** Weakening (2) *)
 
-Lemma sub_has_weakening : (forall m E0 S T, sub m E0 S T -> forall E F G,
-   E0 = E & G ->
+Lemma sub_weakening : forall E F G S T,
+   sub (E & G) S T ->
    okt (E & F & G) ->
-   sub m (E & F & G) S T) /\ (forall E0 p T, has E0 p T -> forall E F G,
-   E0 = E & G ->
-   okt (E & F & G) ->
-   has (E & F & G) p T).
+   sub (E & F & G) S T.
 Proof.
-  apply sub_has_mutind; intros; subst; auto.
-  apply* sub_sel1.
-  apply* sub_sel2.
+  introv Typ. gen F. inductions Typ; introv Ok; auto.
+  apply* sub_sel1. apply* binds_weaken.
+  apply* sub_sel2. apply* binds_weaken.
+  apply* sub_selc1.
+  apply* sub_selc2.
   apply* sub_mem_false.
   apply* sub_mem_true.
   apply_fresh* sub_all as Y. apply_ih_bind* H0.
-  apply* sub_trans_axiom.
-  apply* has_var. apply* binds_weaken.
-  apply* has_mem.
-  apply* has_sub.
+  (*apply* sub_trans.*)
 Qed.
 
-Lemma sub_weakening : forall m E F G S T,
-   sub m (E & G) S T ->
+Lemma sub_weakening1 : forall E F G S T,
+   sub E S T ->
    okt (E & F & G) ->
-   sub m (E & F & G) S T.
-Proof.
-  intros. apply* (proj1 sub_has_weakening).
-Qed.
-
-Lemma sub_weakening1 : forall m E F G S T,
-   sub m E S T ->
-   okt (E & F & G) ->
-   sub m (E & F & G) S T.
+   sub (E & F & G) S T.
 Proof.
   intros.
   assert (E & F & G = E & (F & G) & empty) as A. {
@@ -1016,394 +976,105 @@ Qed.
 
 Section NarrowTrans.
 
+Definition transitivity_on Q := forall E S T,
+  sub E S Q -> sub E Q T -> sub E S T.
+
+Hint Unfold transitivity_on.
+
 Hint Resolve wft_narrow.
 
-Lemma sub_has_narrowing_aux :
-  (forall m E0 S T, sub m E0 S T ->
-   forall Q E F z P,
-   E0 = (E & z ~ Q & F) ->
-   sub notrans E P Q ->
-   sub m (E & z ~ P & F) S T)
-  /\
-  (forall E0 p T, has E0 p T ->
-   forall Q E F z P,
-   E0 = (E & z ~ Q & F) ->
-   sub notrans E P Q ->
-   has (E & z ~ P & F) p T).
+Lemma sub_narrowing_aux : forall Q F E z P S T,
+  transitivity_on Q ->
+  sub (E & z ~ Q & F) S T ->
+  sub E P Q ->
+  sub (E & z ~ P & F) S T.
 Proof.
-  Hint Constructors sub has.
-  apply sub_has_mutind; intros; subst; eauto.
+  introv TransQ SsubT PsubQ.
+  inductions SsubT; introv.
   apply* sub_top.
   apply* sub_refl_sel.
-  apply_fresh* sub_all as Y. apply_ih_bind H0; eauto.
   tests EQ: (x = z).
     lets M: (@okt_narrow Q).
-    apply binds_middle_eq_inv in b. subst.
-    eapply has_sub. apply has_var. apply* M. apply binds_middle_eq.
-      eapply ok_from_okt in o. eapply ok_middle_inv in o. destruct o as [o1 o2]. apply o2.
-      apply* sub_weakening1. auto.
-    apply has_var; eauto. binds_cases b; auto.
-  apply* has_mem.
+    apply (@sub_sel1 P).
+      asserts~ N: (ok (E & z ~ P & F)).
+       lets: ok_middle_inv_r N.
+       apply~ binds_middle_eq.
+      apply TransQ.
+        do_rew* concat_assoc (apply_empty* sub_weakening).
+        binds_get H. auto*.
+    apply* (@sub_sel1 T). binds_cases H; auto.
+  tests EQ: (x = z).
+    lets M: (@okt_narrow Q).
+    apply (@sub_sel2 P) with (S1:=S1).
+      asserts~ N: (ok (E & z ~ P & F)).
+       lets: ok_middle_inv_r N.
+       apply~ binds_middle_eq.
+      apply TransQ.
+        do_rew* concat_assoc (apply_empty* sub_weakening).
+        binds_get H. auto*. auto*.
+    apply* (@sub_sel2 T). binds_cases H; auto.
+  apply* sub_selc1.
+  apply* sub_selc2.
+  apply* sub_mem_false.
+  apply* sub_mem_true.
+  apply_fresh* sub_all as Y. apply_ih_bind* H0.
+  (*apply* sub_trans.*)
 Qed.
 
-Lemma sub_narrowing : forall Q m E F Z P S T,
-  sub notrans E P Q ->
-  sub m (E & Z ~ Q & F) S T ->
-  sub m (E & Z ~ P & F) S T.
+Lemma sub_transitivity : forall Q,
+  transitivity_on Q.
 Proof.
-  intros.
-  apply* (proj1 sub_has_narrowing_aux).
-Qed.
-
-Lemma sub_trans: forall E T1 T2 T3,
-  sub oktrans E T1 T2 ->
-  sub oktrans E T2 T3 ->
-  sub oktrans E T1 T3.
-Proof.
-  introv H12 H23. remember oktrans as m. rewrite Heqm. clear Heqm.
-  induction H12; eauto; inversion H23; subst; eauto 4.
-Qed.
-
-Lemma has_mem_good: forall E t S U,
-  has E t (typ_mem true S) ->
-  has E t (typ_mem false U) ->
-  sub oktrans E S U.
-Proof.
-  introv HS HU.
-  remember (typ_mem true S) as MS.
-  generalize dependent U. generalize dependent S.
-  induction HS; intros; subst; eauto.
-  - generalize dependent S.
-    remember (typ_mem false U) as MU.
-    assert (sub notrans E MU (typ_mem false U)) as A. {
-      subst.
-      eapply (proj2 sub_has_regular) in HU.
-      apply* sub_reflexivity.
-    }
-    clear HeqMU. generalize dependent U.
-    remember (trm_fvar x) as t. generalize dependent x.
-    induction HU; intros; subst; eauto.
-    inversion Heqt. subst. unfold binds in *. rewrite H2 in H1. inversion H1. subst.
-    inversion A; subst. assumption.
-    inversion Heqt.
-    apply* IHHU.
-    
-Lemma sub_untrans_aux: forall E T1 T2 T3,
-  sub notrans E T1 T2 ->
-  sub notrans E T2 T3 ->
-  sub notrans E T1 T3.
-Proof.
-  introv H12 H23. remember notrans as m. gen Heqm.
-  induction H12; intros; subst; eauto; inversion H23; subst; eauto using wft_has_sel;
-  try solve [apply* sub_sel1].
-  - inversion H; subst. inversion H1; subst.
-    unfold binds in *. rewrite H6 in H2. inversion H2.
-    inversion H4
-  - apply* sub_top. apply* wft_has_sel.
-  - apply*
-Qed.
-
-Inductive notvar : typ -> Prop :=
-  | notvar_top   : notvar typ_top
-  | notvar_mem   : forall b T, notvar (typ_mem b T)
-  | notvar_all   : forall T1 T2, notvar (typ_all T1 T2).
-
-Hint Constructors notvar.
-
-Lemma sub_trans_notvar : forall E T1 T2 T3,
-  notvar T2 ->
-  sub notrans E T1 T2 ->
-  sub notrans E T2 T3 ->
-  sub notrans E T1 T3.
-Proof.
-  introv Hnotsel H12 H23.
-  inversion Hnotsel; subst.
-  - (* case top *)
-    inversion H23; subst.
-    + apply* sub_top.
-    + apply* sub_sel2.
-  - (* case mem *)
-    inversion H23; subst.
-    + apply* sub_top.
-    + apply* sub_sel2.
-    + inversion H12; subst.
-      * eapply sub_sel1; eauto.
-      * eapply sub_mem_false; eauto using sub_trans, sub_trans_ok.
-      * eapply sub_mem_false; eauto using sub_trans, sub_trans_ok.
-    + inversion H12; subst.
-      * eapply sub_sel1; eauto.
-      * eapply sub_mem_true; eauto using sub_trans, sub_trans_ok.
-  - (* case all *)
-    inversion H12; inversion H23; subst; auto.
-    + apply* sub_sel2; eauto using sub_trans, sub_trans_ok.
-    + apply* sub_sel1; eauto using sub_trans, sub_trans_ok.
-    + apply* sub_sel2; eauto using sub_trans, sub_trans_ok.
-    + apply sub_all with (L:=L \u L0); eauto using sub_trans.
-      intros Y Fr.
-      apply sub_trans with (T2:=(T4 open_t_var Y)).
-      assert ((E & Y ~ T6) = (E & Y ~ T6 & empty)) as A. {
-        rewrite concat_empty_r. reflexivity.
-      }
-      rewrite A.
-      apply* (@sub_narrowing T0).
-      rewrite concat_empty_r.
-      eauto.
-      eauto.
-Qed.
-
-Inductive follow_ub : env -> typ -> typ -> Prop :=
-  | follow_ub_nil : forall E T,
-      wft E T ->
-      follow_ub E T T
-  | follow_ub_cons : forall E p Hi T,
-      has E p (typ_mem false Hi) ->
-      follow_ub E Hi T ->
-      follow_ub E (typ_sel p) T.
-
-Inductive follow_lb : env -> typ -> typ -> Prop :=
-  | follow_lb_nil : forall E T,
-      wft E T ->
-      follow_lb E T T
-  | follow_lb_cons : forall E p Lo T,
-      has E p (typ_mem true Lo) ->
-      follow_lb E (typ_sel p) T ->
-      follow_lb E Lo T.
-
-Hint Constructors follow_ub.
-Hint Constructors follow_lb.
-
-Lemma follow_lb_reg : forall E T1 T2,
-  follow_lb E T1 T2 ->
-  wft E T1 /\ wft E T2.
-Proof.
-  introv H. induction H; auto.
-  split.
-  apply (proj2 sub_has_regular) in H. destruct H as [? [? A]]. inversion A; subst. assumption.
-  inversion IHfollow_lb. auto.
-Qed.
-
-Lemma invert_follow_lb : forall E T1 T2,
-  follow_lb E T1 T2 ->
-  T1 = T2 \/
-  exists p1 p2 Lo, (typ_sel p2) = T2 /\
-    has E p1 (typ_mem true Lo)  /\
-    sub oktrans E T1 Lo /\
-    follow_lb E (typ_sel p1) (typ_sel p2).
-Proof.
-  intros.
-  induction H.
-  auto.
-  destruct IHfollow_lb as [IH | IH].
-  subst.
-  right. repeat eexists; eauto.
-    eapply (proj2 sub_has_regular) in H. destruct H as [Hok [Hwf1 Hwf2]].
-    eapply sub_trans_ok. apply sub_reflexivity. apply Hok.
-    inversion Hwf2; subst. assumption.
-  right.
-    destruct IH as [p1 [p2 [Lo' [Heq [IH1 [IH2 IH3]]]]]].
-    subst.
-    exists p p2 Lo. splits*.
-    eapply (proj2 sub_has_regular) in H. destruct H as [Hok [Hwf1 Hwf2]].
-    eapply sub_trans_ok. apply sub_reflexivity. apply Hok.
-    inversion Hwf2; subst. assumption.
-Qed.
-
-Definition st_middle (E: env) (B C: typ) : Prop :=
-  B = C \/
-  sub notrans E typ_top C \/
-  (notvar B /\ sub notrans E B C).
-
-Definition chain (E: env) (A D: typ): Prop :=
-  (exists B C, follow_ub E A B /\ st_middle E B C /\ follow_lb E C D).
-
-Lemma empty_chain: forall E T, wft E T -> chain E T T.
-Proof.
-  intros.
-  unfold chain. unfold st_middle.
-  exists T T.
-  auto.
-Qed.
-
-Lemma chain3sub: forall E C1 C2 D,
-  sub notrans E C1 C2 ->
-  follow_lb E C2 D ->
-  sub notrans E C1 D.
-Proof.
-  introv Hst Hflb.
-  induction Hflb.
-  assumption.
-  apply IHHflb.
-  eapply sub_sel2; eauto using sub_trans_ok.
-Qed.
-
-Lemma chain2sub: forall E B1 B2 C D,
-  sub notrans E B1 B2 ->
-  st_middle E B2 C ->
-  follow_lb E C D ->
-  sub notrans E B1 D.
-Proof.
-  introv Hst Hm Hflb.
-  unfold st_middle in Hm.
-  destruct Hm as [Hm | [Hm | [Hm1 Hm2]]]; subst.
-  apply (chain3sub Hst Hflb).
-  apply chain3sub with (C2:=C).
-    apply sub_trans_notvar with (T2:=typ_top); auto.
-    apply Hflb.
-  apply chain3sub with (C2:=C).
-    apply sub_trans_notvar with (T2:=B2); auto.
-    apply Hflb.
-Qed.
-
-
-Lemma chain1sub: forall E A B C D,
-  okt E ->
-  follow_ub E A B ->
-  st_middle E B C ->
-  follow_lb E C D ->
-  sub notrans E A D.
-Proof.
-  introv Hok Hfub Hm Hflb.
-  induction Hfub.
-  apply chain2sub with (B2:=T) (C:=C); try assumption.
-    apply sub_reflexivity; auto.
-  apply* sub_sel1.
-Qed.
-
-Lemma prepend_chain: forall E A1 A2 D,
-  sub oktrans E A1 A2 ->
-  chain E A2 D ->
-  chain E A1 D.
-Proof. admit. Qed.
 (*
-  fix 5.
-  introv Hsub Hch.
-  unfold chain in *. unfold st_middle in *.
-  inversion Hsub; inversion H; subst.
-  - (* case top *)
-    destruct Hch as [B [C [Hch1 [Hch2 Hch3]]]].
-    inversion Hch1; subst.
-    destruct Hch2 as [Hch2 | [Hch2 | [Hch2a Hch2b]]]; subst.
-    + exists A1 typ_top. auto 10.
-    + exists A1 C. auto 10.
-    + exists A1 C. auto 10.
-  - (* case refl_sel *)
-    assumption.
-  - (* case sel1 *)
-    admit.
-    (*
-    set (IH := (prepend_chain E (typ_sel t) A2 D Hsub Hch)).
-    destruct IH as [B [C [IH1 [IH2 IH3]]]].
-    exists B C.
-    split.
-    assumption.
-    split; assumption.
-    *)
-  - (* case sel2 *)
-    set (Hch' := Hch).
-    destruct Hch' as [B [C [Hch1 [Hch2 Hch3]]]].
-    inversion Hch1; subst.
-    + destruct Hch2 as [Hch2 | [Hch2 | [Hch2a Hch2b]]].
-      subst.
-      apply (prepend_chain E A1 (typ_sel t) D Hsub).
-      exists (typ_sel t) (typ_sel t).
-      set (Hflb := (follow_lb_cons H0 Hch3)).
-      auto.
-      exists A1 C.
-      splits.
-      apply follow_ub_nil. auto.
-      right. left. apply Hch2. apply Hch3.
-      inversion Hch2a.
-    + apply (prepend_chain E A1 (typ_sel t) D Hsub).
-      exists B C.
-      splits.
-      assumption.
-      assumption.
-      assumption.
-  - (* case mem_false *)
-    admit.
-  - (* case mem_true *)
-    admit.
-  - (* case all *)
-    destruct Hch as [B [C [Hch1 [Hch2 Hch3]]]].
-    inversion Hch1; subst.
-    exists (typ_all S1 S2) C.
-    destruct Hch2 as [Hch2 | [Hch2 | [Hch2a Hch2b]]].
-    subst.
-    auto 10.
-    auto 10.
-    set (Hst := (sub_trans_notvar (notvar_all _ _) H Hch2b)).
-    auto 10.
-  - (* case trans_ok *)
-    apply (prepend_chain E _ _ _ H (prepend_chain E _ _ _ H0 Hch)).
-  - (* case trans *)
-    apply (prepend_chain E _ _ _ H (prepend_chain E _ _ _ H0 Hch)).
+  intro Q. introv SsubQ QsubT.
+  eapply sub_trans; eauto.
+*)
+admit.
 Qed.
- *)
 
-Lemma sub_trans_pushback : forall E T1 T3,
-  sub oktrans E T1 T3 ->
-  sub notrans E T1 T3.
+Lemma sub_narrowing : forall Q E F Z P S T,
+  sub E P Q ->
+  sub (E & Z ~ Q & F) S T ->
+  sub (E & Z ~ P & F) S T.
 Proof.
-  introv Hst.
-  inversion Hst; subst.
-  assumption.
-  assert (wft E T3) as HwfT3 by auto.
-  assert (okt E) as Hok by auto.
-  set (Hch := (prepend_chain H (prepend_chain H0 (empty_chain HwfT3)))).
-  unfold chain in Hch.
-  destruct Hch as [B [C [Hch1 [Hch2 Hch3]]]].
-  apply (chain1sub Hok Hch1 Hch2 Hch3).
+  intros.
+  apply* sub_narrowing_aux.
+  apply* sub_transitivity.
 Qed.
 
 End NarrowTrans.
 
-Lemma contra_all_mem: forall E V T1 U,
-  sub E (typ_all V T1) (typ_mem false U) ->
-  False.
-Proof.
-  introv Hsub. remember (typ_all V T1) as LHS. remember (typ_mem false U) as RHS.
-  gen HeqLHS. gen HeqRHS. gen V T1 U.
-  induction Hsub; intros; try solve [inversion HeqRHS]; try solve [inversion HeqLHS].
-  subst. inversion Hsub1; subst.
-  assert (H
-  eapply IHHsub2. reflexivity.
-Lemma mem_inv_val: forall u Q U E F,
-  value u ->
-  typing E u Q ->
-  sub (E & F) Q (typ_mem false U) ->
-  exists S, sub (E & F) S U /\ trm_mem S = u.
-Proof.
-  introv VU TU Sub. gen VU. generalize dependent F. generalize dependent U.
-  induction TU; intros; subst; try solve [inversion VU].
-  inversion Sub
-
-Lemma mem_inv: forall u Q U E F,
-  (value u \/ (exists x, trm_fvar x = u)) ->
-  typing E u Q ->
-  sub (E & F) Q (typ_mem false U) ->
-  (exists S, sub (E & F) S U /\
-  (trm_mem S = u \/ (exists x, trm_fvar x = u /\ binds x S E))).
-Proof.
-  introv VU.  destruct VU as [VU | [x Eq]].
-
 (* ********************************************************************** *)
-(** Substitution preserves subtyping (10) *)
+(** Type substitution preserves subtyping (10) *)
 
-Lemma sub_through_subst : forall Q E F Z S T u,
+Definition subst_tb (Z : var) (P : typ) (b : typ) : typ :=
+  subst_t Z (trm_mem P) b.
+
+Ltac unsimpl_map_bind :=
+  match goal with |- context [ ?B (subst_t ?Z (trm_mem ?P) ?U) ] =>
+    unsimpl ((subst_tb Z P) (B U)) end.
+
+Tactic Notation "unsimpl_map_bind" "*" :=
+  unsimpl_map_bind; auto*.
+
+Lemma sub_through_subst_tb : forall Q E F Z S T P,
   sub (E & Z ~ Q & F) S T ->
-  (value u \/ exists x, trm_fvar x = u) -> typing E u Q ->
-  sub (E & map (subst_t Z u) F) (subst_t Z u S) (subst_t Z u T).
+  sub E (typ_mem true P) Q ->
+  sub (E & map (subst_tb Z P) F) (subst_tb Z P S) (subst_tb Z P T).
 Proof.
-  introv SsubT VU TU.
-  assert (wfe E u) as WU by solve [apply typing_regular in TU; auto*].
+  introv SsubT PsubQ.
+  assert (wft E P) as WfP. {
+    apply sub_regular in PsubQ. destruct PsubQ as [? [A ?]]. inversion A; subst.
+    assumption.
+  }
   inductions SsubT; introv.
   - apply* sub_top.
-  - simpl. apply* sub_refl_sel.
-    assert (typ_sel (subst_e Z u t) = subst_t Z u (typ_sel t)) as A by auto.
+  - repeat unfold subst_tb at 2; simpl subst_t. apply* sub_refl_sel.
+    assert (typ_sel (subst_e Z (trm_mem P) t) = subst_tb Z P (typ_sel t)) as A. {
+      unfold subst_tb. simpl. reflexivity.
+    }
     rewrite A. auto*.
-  - simpl. case_var.
+  - repeat unfold subst_tb at 2; simpl subst_t. case_var.
     + apply binds_middle_eq_inv in H; eauto. subst.
-      apply sub_selc1.
       assert (sub (E & map (subst_tb Z P) F) (typ_mem true P) (typ_mem false (subst_t Z (trm_mem P) U))) as A. {
         apply (@sub_transitivity Q).
         apply_empty* sub_weakening.
